specs/HMAC_DRBG_generate_algorithm.v
@@ -8,18 +8,24 @@ Require Import DRBG_generate_algorithm_result.
 Function HMAC_DRBG_generate_helper (HMAC: list Z -> list Z -> list Z) (key v: list Z) (requested_number_of_bytes: Z) {measure Z.to_nat requested_number_of_bytes}: (list Z * list Z) :=
   if Z.geb 0 requested_number_of_bytes then (v, [])
   else
-    let v := HMAC key v in
+    let v := HMAC v key in
     let temp := v in
     let len := 32%nat in (* TODO get this from property of HMAC *)
     let (v, rest) := HMAC_DRBG_generate_helper HMAC key v (requested_number_of_bytes - (Z.of_nat len)) in
-    (v, temp ++ v).
+    (v, temp ++ rest). 
 Proof.
   intros. rewrite Z2Nat.inj_sub by omega.
   rewrite Nat2Z.id.
-  assert ((0 <? requested_number_of_bytes) = true). admit. (* TODO *)
+  assert ((0 <? requested_number_of_bytes) = true).
+  * 
+    rewrite Z.ltb_antisym.
+    rewrite <- Z.geb_leb.
+    rewrite teq.
+    auto.
+  *
   apply Zlt_is_lt_bool in H.
   apply Z2Nat.inj_lt in H; omega.
-Qed.
+Defined.
 
 Fixpoint leftmost_items {A: Type} (items: list A) (count: Z) :=
   if Z.geb 0 count then []
@@ -29,7 +35,7 @@ Fixpoint leftmost_items {A: Type} (items: list A) (count: Z) :=
       | hd::tl => hd::leftmost_items tl (count - 1)
     end.
 
-Definition HMAC_DRBG_generate_algorithm (reseed_interval: Z) (HMAC: list Z -> list Z -> list Z) (working_state: DRBG_working_state) (requested_number_of_bytes: Z) (additional_input: list Z): DRBG_generate_algorithm_result :=
+Definition HMAC_DRBG_generate_algorithm (HMAC: list Z -> list Z -> list Z) (reseed_interval: Z) (working_state: DRBG_working_state) (requested_number_of_bytes: Z) (additional_input: list Z): DRBG_generate_algorithm_result :=
   let '(v, key, reseed_counter) := working_state in
   if Z.gtb reseed_counter reseed_interval then generate_algorithm_reseed_required
   else
